\newpage
Use (8) to solve the diffusion equation if $\phi(x) = e^{3x}$ . (You may also use
Exercises 6 and 7 below.)

\begin{gather*}
	\frac{ 1 }{\sqrt{ 4 \pi k t } }\int_{-\infty }^{\infty }e^{-(x-y)^2/4kt}(e^{3y})\ dy = \frac{ 1 }{\sqrt{ 4 \pi k t }}\int_{-\infty }^{\infty } e^{\frac{-y^2+2xy-x^2+12kty  }{4kt }}dy\\
	\frac{ e^{-(x^2)/4kt} }{\sqrt{ 4\pi kt }}\int_{-\infty }^{\infty }e^{-(y^2-y(12kt+2x))/4kt}dy=\frac{ e^{-x^2} }{\sqrt{ 4\pi kt }}\int_{-\infty }^{\infty }e^{-((y-(12kt+2x)/2)^2-(12kt+2x)^2/4)/4kt}dy\\
\frac{ e^{(-x^2+(6kt+x)^2)/4kt}}{\sqrt{ 4\pi kt }}\int_{-\infty }^{\infty }e^{-(y-(12kt+2x)/2)^2/4kt}dy\end{gather*}
$$ \text{Let } p=f(y)=\frac{(y-(6kt+x)/2) }{\sqrt{ 4kt}}, t,k\text{ ought be positive so should be safe. Jacobian }\frac{\partial y}{\partial p }=\sqrt{ 4kt } \text{ so we get}:$$
\begin{gather*}
\frac{ e^{(-x^2+(6kt+x)^2)/4kt}}{\sqrt{ 4\pi kt }}\sqrt{ 4kt }\int_{-\infty }^{\infty }e^{-(p^2)}dp=\frac{ e^{(-x^2+(6kt+x)^2)/4kt}}{\sqrt{ \pi  }}\left[  \sqrt{ \pi } \right]\\
e^{(-x^2+36(k^2t^2)+12ktx+x^2)/4kt}=e^{9kt+3x}
\end{gather*}
